Adjust Sorts

matching-logic/src/Theories/Sorts.v
@@ -57,39 +57,41 @@ Section sorts.
     |}.
 
   Definition patt_forall_of_sort (sort phi : Pattern) : Pattern :=
-    patt_forall ((patt_in (patt_bound_evar 0) (patt_inhabitant_set (nest_ex sort))) ---> phi).
+    patt_forall ((patt_in (patt_bound_evar 0) (patt_inhabitant_set sort)) ---> phi).
 
   Definition patt_exists_of_sort (sort phi : Pattern) : Pattern :=
-    patt_exists ((patt_in (patt_bound_evar 0) (patt_inhabitant_set (nest_ex sort))) and phi).
+    patt_exists ((patt_in (patt_bound_evar 0) (patt_inhabitant_set sort)) and phi).
 
   Lemma bevar_subst_forall_of_sort s ψ (wfcψ : well_formed_closed ψ) db ϕ :
-    bevar_subst (patt_forall_of_sort s ϕ) ψ db = patt_forall_of_sort (bevar_subst s ψ db) (bevar_subst ϕ ψ (db+1)).
-  Proof.
+    bevar_subst (patt_forall_of_sort s ϕ) ψ db = patt_forall_of_sort (bevar_subst s ψ (S db)) (bevar_subst ϕ ψ (S db)).
+  Proof. reflexivity. Qed.
+
+  (*  TODO: deprecated
     unfold patt_forall_of_sort.
     repeat (rewrite simpl_bevar_subst';[assumption|]).
     (* TODO rewrite all _+1 to 1+_ *)
     rewrite PeanoNat.Nat.add_comm. simpl.
-    rewrite bevar_subst_nest_ex_aux.
-    { unfold well_formed_closed in wfcψ. destruct_and!. assumption. }
     simpl.
     rewrite PeanoNat.Nat.sub_0_r.
     reflexivity.
-  Qed.
+  Qed. *)
 
   Lemma bsvar_subst_forall_of_sort s ψ (wfcψ : well_formed_closed ψ) db ϕ :
     bsvar_subst (patt_forall_of_sort s ϕ) ψ db = patt_forall_of_sort (bsvar_subst s ψ db) (bsvar_subst ϕ ψ db).
-  Proof.
+  Proof. reflexivity. Qed.
+(*  TODO: deprecated
     unfold patt_forall_of_sort.
     repeat (rewrite simpl_bsvar_subst';[assumption|]).
     simpl.
     rewrite bsvar_subst_nest_ex_aux_comm.
     { unfold well_formed_closed in wfcψ. destruct_and!. assumption. }
     reflexivity.
-  Qed.
+  Qed.*)
 
   Lemma bevar_subst_exists_of_sort s ψ (wfcψ : well_formed_closed ψ) db ϕ :
-    bevar_subst (patt_exists_of_sort s ϕ) ψ db = patt_exists_of_sort (bevar_subst s ψ db) (bevar_subst ϕ ψ (db+1)).
-  Proof.
+    bevar_subst (patt_exists_of_sort s ϕ) ψ db = patt_exists_of_sort (bevar_subst s ψ (S db)) (bevar_subst ϕ ψ (S db)).
+  Proof. reflexivity. Qed.
+(*  TODO: deprecated
     unfold patt_exists_of_sort.
     repeat (rewrite simpl_bevar_subst';[assumption|]).
     (* TODO rewrite all _+1 to 1+_ *)
@@ -100,18 +102,19 @@ Section sorts.
     simpl.
     rewrite PeanoNat.Nat.sub_0_r.
     reflexivity.
-  Qed.
+  Qed.*)
 
   Lemma bsvar_subst_exists_of_sort s ψ (wfcψ : well_formed_closed ψ) db ϕ :
     bsvar_subst (patt_exists_of_sort s ϕ) ψ db = patt_exists_of_sort (bsvar_subst s ψ db) (bsvar_subst ϕ ψ db).
-  Proof.
-    unfold patt_exists_of_sort.
+  Proof. reflexivity. Qed.
+(* TODO: deprecated
+     unfold patt_exists_of_sort.
     repeat (rewrite simpl_bsvar_subst';[assumption|]).
     simpl.
     rewrite bsvar_subst_nest_ex_aux_comm.
     { unfold well_formed_closed in wfcψ. destruct_and!. assumption. }
     reflexivity.
-  Qed.
+  Qed. *)
     
   #[global]
    Instance EBinder_forall_of_sort s : EBinder (patt_forall_of_sort s) _ _:=
@@ -130,27 +133,27 @@ Section sorts.
   (* TODO patt_forall_of_sort and patt_exists_of_sorts are duals - a lemma *)
 
   (* TODO a lemma about patt_forall_of_sort *)
-  
+
   Definition patt_total_function(phi from to : Pattern) : Pattern :=
-    patt_forall_of_sort from (patt_exists_of_sort (nest_ex to) (patt_equal (patt_app (nest_ex (nest_ex phi)) b1) b0)).
+    patt_forall_of_sort from (patt_exists_of_sort to (patt_equal (patt_app phi b1) b0)).
 
   Definition patt_partial_function(phi from to : Pattern) : Pattern :=
-    patt_forall_of_sort from (patt_exists_of_sort (nest_ex to) (patt_subseteq (patt_app (nest_ex (nest_ex phi)) b1) b0)).
+    patt_forall_of_sort from (patt_exists_of_sort to (patt_subseteq (patt_app phi b1) b0)).
 
 
   (* Assuming `f` is a total function, says it is injective on given domain. Does not quite work for partial functions. *)
   Definition patt_total_function_injective f from : Pattern :=
-    patt_forall_of_sort from (patt_forall_of_sort (nest_ex from) (patt_imp (patt_equal (patt_app (nest_ex (nest_ex f)) b1) (patt_app (nest_ex (nest_ex f)) b0)) (patt_equal b1 b0))).
+    patt_forall_of_sort from (patt_forall_of_sort from (patt_imp (patt_equal (patt_app f b1) (patt_app f b0)) (patt_equal b1 b0))).
 
   (* Assuming `f` is a partial function, says it is injective on given domain. Works for total functions, too. *)
   Definition patt_partial_function_injective f from : Pattern :=
     patt_forall_of_sort
       from
       (patt_forall_of_sort
-         (nest_ex from)
+         from
          (patt_imp
-            (patt_not (patt_equal (patt_app (nest_ex (nest_ex f)) b1) patt_bott ))
-            (patt_imp (patt_equal (patt_app (nest_ex (nest_ex f)) b1) (patt_app (nest_ex (nest_ex f)) b0)) (patt_equal b1 b0)))).
+            (patt_not (patt_equal (patt_app f b1) patt_bott ))
+            (patt_imp (patt_equal (patt_app f b1) (patt_app f b0)) (patt_equal b1 b0)))).
   
 
   Section with_model.
@@ -165,13 +168,14 @@ Section sorts.
     Lemma pattern_interpretation_forall_of_sort_predicate s ϕ ρₑ ρₛ:
       let x := fresh_evar ϕ in
       M_predicate M (evar_open 0 x ϕ) ->
+      well_formed_closed_ex_aux s 0 ->
       pattern_interpretation ρₑ ρₛ (patt_forall_of_sort s ϕ) = ⊤
       <-> (∀ m : Domain M, m ∈ Minterp_inhabitant s ρₑ ρₛ ->
                            pattern_interpretation (update_evar_val x m ρₑ) ρₛ (evar_open 0 x ϕ) = ⊤).
     Proof.
-      intros x Hpred.
+      intros x Hpred Hwfs.
       unfold patt_forall_of_sort.
-      assert (Hsub: is_subformula_of_ind ϕ (patt_in b0 (patt_inhabitant_set (nest_ex s)) ---> ϕ)).
+      assert (Hsub: is_subformula_of_ind ϕ (patt_in b0 (patt_inhabitant_set s) ---> ϕ)).
       { apply sub_imp_r. apply sub_eq. reflexivity.  }
       rewrite pattern_interpretation_forall_predicate.
       2: {
@@ -185,8 +189,8 @@ Section sorts.
           eapply evar_fresh_in_subformula. apply Hsub. apply set_evar_fresh_is_fresh.
       }
       subst x.
-      remember (patt_in b0 (patt_inhabitant_set (nest_ex s)) ---> ϕ) as Bigϕ.
-      assert (Hfresh: fresh_evar Bigϕ ∉ free_evars (patt_sym (inj inhabitant) $ (nest_ex s))).
+      remember (patt_in b0 (patt_inhabitant_set s) ---> ϕ) as Bigϕ.
+      assert (Hfresh: fresh_evar Bigϕ ∉ free_evars (patt_sym (inj inhabitant) $ s)).
       { rewrite HeqBigϕ.
         unfold patt_inhabitant_set.
         fold (evar_is_fresh_in (fresh_evar (patt_in b0 (sym inhabitant $ s) ---> ϕ)) (patt_sym (inj inhabitant) $ s)).
@@ -203,7 +207,7 @@ Section sorts.
 
       remember (patt_in b0 (patt_inhabitant_set s) ---> ϕ) as Bigϕ'.
       assert (HfreeBigϕ: free_evars Bigϕ = free_evars Bigϕ').
-      { subst. simpl. unfold nest_ex. rewrite free_evars_nest_ex_aux. reflexivity. }
+      { subst. reflexivity. }
       assert (HfreshBigϕ: fresh_evar Bigϕ = fresh_evar Bigϕ').
       { unfold fresh_evar. rewrite HfreeBigϕ. reflexivity. }
       clear HfreeBigϕ.
@@ -221,67 +225,68 @@ Section sorts.
         specialize (H m).
         (*rewrite -interpretation_fresh_evar_subterm.*)
         rewrite -(@interpretation_fresh_evar_subterm _ _ _ Bigϕ).
-        rewrite HeqBigϕ in H.
-        rewrite evar_open_imp in H.
-        rewrite -HeqBigϕ in H.
         assumption.
-        rewrite {3}HeqBigϕ in H.
-        eapply pattern_interpretation_impl_MP.
-        apply H.
-        simpl. fold evar_open.
+        rewrite -> HeqBigϕ, -> HeqBigϕ' in H.
+        rewrite evar_open_imp in H.
+        rewrite <- HeqBigϕ', <- HeqBigϕ in H.
+
+        apply pattern_interpretation_impl_MP with (ϕ₁ := evar_open 0 (fresh_evar Bigϕ) (patt_in b0 (patt_inhabitant_set s))). exact H.
   
         unfold Minterp_inhabitant in H'.
-        pose proof (Hfeip := @free_evar_in_patt _ _ M M_satisfies_theory (fresh_evar Bigϕ) (patt_sym (inj inhabitant) $ evar_open 0 (fresh_evar Bigϕ) (nest_ex s)) (update_evar_val (fresh_evar Bigϕ) m ρₑ) ρₛ).
+        pose proof (Hfeip := @free_evar_in_patt _ _ M M_satisfies_theory (fresh_evar Bigϕ) (patt_sym (inj inhabitant) $ evar_open 0 (fresh_evar Bigϕ) s) (update_evar_val (fresh_evar Bigϕ) m ρₑ) ρₛ).
         destruct Hfeip as [Hfeip1 _]. apply Hfeip1. clear Hfeip1.
         rewrite update_evar_val_same.
         clear H. unfold sym in H'.
         unfold Ensembles.In.
         
         rewrite pattern_interpretation_app_simpl.
-        rewrite pattern_interpretation_evar_open_nest_ex. apply Hfrs.
         rewrite pattern_interpretation_sym_simpl.
 
         rewrite pattern_interpretation_app_simpl in H'.
         rewrite pattern_interpretation_sym_simpl in H'.
-        apply H'.
+
+        rewrite evar_open_not_occur; [auto|].
+        rewrite pattern_interpretation_free_evar_independent; [solve_free_evars_inclusion 5 | exact H' ].
 
       - intros H m.
-        pose proof (Hfeip := @free_evar_in_patt _ _ M M_satisfies_theory (fresh_evar Bigϕ) (patt_sym (inj inhabitant) $ evar_open 0 (fresh_evar Bigϕ) (nest_ex s)) (update_evar_val (fresh_evar Bigϕ) m ρₑ) ρₛ).
+        pose proof (Hfeip := @free_evar_in_patt _ _ M M_satisfies_theory (fresh_evar Bigϕ) (patt_sym (inj inhabitant) $ evar_open 0 (fresh_evar Bigϕ) s) (update_evar_val (fresh_evar Bigϕ) m ρₑ) ρₛ).
         destruct Hfeip as [_ Hfeip2].
-        rewrite {3}HeqBigϕ.
-        unfold evar_open. simpl_bevar_subst. simpl.
+        unfold evar_open. simpl.
+        rewrite -> HeqBigϕ, -> HeqBigϕ'.
         apply pattern_interpretation_predicate_impl.
         apply T_predicate_in. apply M_satisfies_theory.
-        intros H1.
+        intros H1. fold bevar_subst in *. rewrite -> HeqBigϕ, -> HeqBigϕ' in Hfeip2.
         specialize (Hfeip2 H1). clear H1.
         specialize (H m).
         rewrite -(@interpretation_fresh_evar_subterm _ _ _ Bigϕ) in H.
-        apply Hsub. apply H. clear H.
+        apply Hsub.
+        rewrite -> HeqBigϕ, -> HeqBigϕ' in H.
+        apply H. clear H.
         
         unfold Minterp_inhabitant.
         unfold Ensembles.In in Hfeip2. unfold sym.
-
-
         rewrite pattern_interpretation_app_simpl in Hfeip2.
-        rewrite pattern_interpretation_evar_open_nest_ex in Hfeip2. apply Hfrs.
         rewrite pattern_interpretation_sym_simpl in Hfeip2.
 
         rewrite pattern_interpretation_app_simpl.
         rewrite pattern_interpretation_sym_simpl.
         rewrite update_evar_val_same in Hfeip2.
-        apply Hfeip2.
+        rewrite evar_open_not_occur in Hfeip2; [auto|].
+        rewrite pattern_interpretation_free_evar_independent in Hfeip2; auto.
+        unfold evar_is_fresh_in, fresh_evar. cbn.
+        set_solver.
     Qed.
 
     Lemma pattern_interpretation_exists_of_sort_predicate s ϕ ρₑ ρₛ:
       let x := fresh_evar ϕ in
-      M_predicate M (evar_open 0 x ϕ) ->
+      M_predicate M (evar_open 0 x ϕ) -> well_formed_closed_ex_aux s 0 ->
       pattern_interpretation ρₑ ρₛ (patt_exists_of_sort s ϕ) = ⊤
       <-> (∃ m : Domain M, m ∈ Minterp_inhabitant s ρₑ ρₛ /\
                            pattern_interpretation (update_evar_val x m ρₑ) ρₛ (evar_open 0 x ϕ) = ⊤).
     Proof.
-      intros x Hpred.
+      intros x Hpred WFs.
       unfold patt_exists_of_sort.
-      assert (Hsub: is_subformula_of_ind ϕ (patt_in b0 (patt_inhabitant_set (nest_ex s)) and ϕ)).
+      assert (Hsub: is_subformula_of_ind ϕ (patt_in b0 (patt_inhabitant_set s) and ϕ)).
       { unfold patt_and. unfold patt_or.  apply sub_imp_l. apply sub_imp_r. apply sub_imp_l. apply sub_eq. reflexivity. }
       rewrite -> pattern_interpretation_exists_predicate_full.
       2: {
@@ -295,8 +300,8 @@ Section sorts.
           eapply evar_fresh_in_subformula. apply Hsub. apply set_evar_fresh_is_fresh.
       }
       subst x.
-      remember (patt_in b0 (patt_inhabitant_set (nest_ex s)) and ϕ) as Bigϕ.
-      assert (Hfresh: fresh_evar Bigϕ ∉ free_evars (patt_sym (inj inhabitant) $ (nest_ex s))).
+      remember (patt_in b0 (patt_inhabitant_set s) and ϕ) as Bigϕ.
+      assert (Hfresh: fresh_evar Bigϕ ∉ free_evars (patt_sym (inj inhabitant) $ s)).
       { rewrite HeqBigϕ.
         unfold patt_inhabitant_set.
         fold (evar_is_fresh_in (fresh_evar (patt_in b0 (sym inhabitant $ s) and ϕ)) (patt_sym (inj inhabitant) $ s)).
@@ -315,7 +320,7 @@ Section sorts.
 
       remember (patt_in b0 (patt_inhabitant_set s) and ϕ) as Bigϕ'.
       assert (HfreeBigϕ: free_evars Bigϕ = free_evars Bigϕ').
-      { subst. simpl. unfold nest_ex. rewrite free_evars_nest_ex_aux. reflexivity. }
+      { subst. reflexivity. }
       assert (HfreshBigϕ: fresh_evar Bigϕ = fresh_evar Bigϕ').
       { unfold fresh_evar. rewrite HfreeBigϕ. reflexivity. }
       clear HfreeBigϕ.
@@ -333,36 +338,40 @@ Section sorts.
         exists m.
         rewrite -(@interpretation_fresh_evar_subterm _ _ _ Bigϕ).
         assumption.
-        rewrite {3}HeqBigϕ in H.
+        simpl in H. rewrite -> HeqBigϕ, -> HeqBigϕ' in H.
 
         apply pattern_interpretation_and_full in H.
-        fold evar_open in H.
+        fold bevar_subst in H.
         destruct H as [H1 H2].
-        split. 2: apply H2. clear H2.
+        split. 2:rewrite -> HeqBigϕ, -> HeqBigϕ'; apply H2. clear H2.
         unfold Minterp_inhabitant.
-        pose proof (Hfeip := @free_evar_in_patt _ _ M M_satisfies_theory (fresh_evar Bigϕ) (patt_sym (inj inhabitant) $ evar_open 0 (fresh_evar Bigϕ) (nest_ex s)) (update_evar_val (fresh_evar Bigϕ) m ρₑ) ρₛ).
+        pose proof (Hfeip := @free_evar_in_patt _ _ M M_satisfies_theory (fresh_evar Bigϕ) (patt_sym (inj inhabitant) $ evar_open 0 (fresh_evar Bigϕ) s) (update_evar_val (fresh_evar Bigϕ) m ρₑ) ρₛ).
         destruct Hfeip as [_ Hfeip2].
 
+        rewrite -> HeqBigϕ, -> HeqBigϕ' in Hfeip2.
         apply Hfeip2 in H1. clear Hfeip2.
         rewrite update_evar_val_same in H1.
         unfold sym.
         unfold Ensembles.In in H1.
 
         rewrite pattern_interpretation_app_simpl in H1.
-        rewrite pattern_interpretation_evar_open_nest_ex in H1. apply Hfrs.
         rewrite pattern_interpretation_sym_simpl in H1.
 
         rewrite pattern_interpretation_app_simpl.
         rewrite pattern_interpretation_sym_simpl.
-        apply H1.
+        rewrite evar_open_not_occur in H1; [auto|].
+        rewrite pattern_interpretation_free_evar_independent in H1; auto.
+        unfold evar_is_fresh_in, fresh_evar. cbn.
+        set_solver.
         
-      - intros [m [H1 H2]]. exists m.
-        pose proof (Hfeip := @free_evar_in_patt _ _ M M_satisfies_theory (fresh_evar Bigϕ) (patt_sym (inj inhabitant) $ evar_open 0 (fresh_evar Bigϕ) (nest_ex s)) (update_evar_val (fresh_evar Bigϕ) m ρₑ) ρₛ).
+      - intros [m [H1 H2] ]. exists m.
+        pose proof (Hfeip := @free_evar_in_patt _ _ M M_satisfies_theory (fresh_evar Bigϕ) (patt_sym (inj inhabitant) $ evar_open 0 (fresh_evar Bigϕ) s) (update_evar_val (fresh_evar Bigϕ) m ρₑ) ρₛ).
         destruct Hfeip as [Hfeip1 _].
-        rewrite {3}HeqBigϕ.
-        apply pattern_interpretation_and_full. fold evar_open.
+        rewrite -> HeqBigϕ, -> HeqBigϕ'.
+        apply pattern_interpretation_and_full. fold bevar_subst.
         split.
-        + apply Hfeip1. clear Hfeip1.
+        + rewrite -> HeqBigϕ, -> HeqBigϕ' in Hfeip1.
+          apply Hfeip1. clear Hfeip1.
           unfold Ensembles.In.
           rewrite -> update_evar_val_same.
           unfold Minterp_inhabitant in H1. unfold sym in H1.
@@ -371,12 +380,12 @@ Section sorts.
           rewrite pattern_interpretation_sym_simpl in H1.
 
           rewrite pattern_interpretation_app_simpl.
-          rewrite pattern_interpretation_evar_open_nest_ex. apply Hfrs.
           rewrite pattern_interpretation_sym_simpl.
-          apply H1.
+          rewrite evar_open_not_occur; [auto|].
+          rewrite pattern_interpretation_free_evar_independent; [set_solver | exact H1 ].
         + rewrite -(@interpretation_fresh_evar_subterm _ _ _ Bigϕ) in H2.
           apply Hsub.
-          apply H2.
+          rewrite -> HeqBigϕ, -> HeqBigϕ' in H2. apply H2.
     Qed.
 
 
@@ -425,18 +434,18 @@ Section sorts.
     Hint Resolve M_predicate_forall_of_sort : core.
     
     Lemma interp_total_function f s₁ s₂ ρₑ ρₛ :
+      well_formed_closed_ex_aux s₁ 0 -> well_formed_closed_ex_aux s₂ 0 ->
+      well_formed_closed_ex_aux f 0 ->
       @pattern_interpretation Σ M ρₑ ρₛ (patt_total_function f s₁ s₂) = ⊤ <->
       @is_total_function Σ M f (Minterp_inhabitant s₁ ρₑ ρₛ) (Minterp_inhabitant s₂ ρₑ ρₛ) ρₑ ρₛ.
     Proof.
+      intros WF1 WF2 WFF.
       unfold is_total_function.
-      rewrite pattern_interpretation_forall_of_sort_predicate.
+      rewrite pattern_interpretation_forall_of_sort_predicate; auto.
       2: { eauto. }
 
       unfold evar_open. simpl_bevar_subst.
-      remember (fresh_evar (patt_exists_of_sort (nest_ex s₂) (patt_equal ((nest_ex (nest_ex f)) $ b1) b0))) as x'.
-      rewrite [nest_ex s₂]/nest_ex.
-      rewrite bevar_subst_nest_ex_aux;[reflexivity|]. simpl.
-      rewrite -/(nest_ex s₂).
+      remember (fresh_evar (patt_exists_of_sort s₂ (patt_equal (f $ b1) b0))) as x'.
 
       apply all_iff_morphism.
       unfold pointwise_relation. intros m₁.
@@ -453,36 +462,36 @@ Section sorts.
       rewrite 2!pattern_interpretation_app_simpl.
       rewrite 2!pattern_interpretation_sym_simpl.
       rewrite pattern_interpretation_free_evar_independent.
-      (* two subgoals *)
-      fold (evar_is_fresh_in x' (nest_ex s₂)).
+      { rewrite Heqx'. rewrite bevar_subst_not_occur; [eapply well_formed_closed_ex_aux_ind;
+                               try eassumption; lia|].
+        eapply evar_is_fresh_in_richer.
+        2: apply set_evar_fresh_is_fresh.
+        cbn. rewrite !(left_id_L ∅ union). rewrite !(right_id_L ∅ union).
+        rewrite (idemp_L union). apply union_subseteq_l. } 
 
-      assert (Hfreq: x' = fresh_evar (patt_imp s₂ (nest_ex (nest_ex f)))).
+      assert (Hfreq: x' = fresh_evar (patt_imp s₂ f)).
       { rewrite Heqx'. unfold fresh_evar. apply f_equal. simpl.
-        rewrite 2!free_evars_nest_ex_aux.
         rewrite !(left_id_L ∅ union). rewrite !(right_id_L ∅ union).
         rewrite (idemp_L union). reflexivity.
       }
+      2: { rewrite bevar_subst_not_occur; [eapply well_formed_closed_ex_aux_ind;
+                               try eassumption; lia|auto]. }
 
       rewrite Hfreq.
-      unfold nest_ex.
-      unfold evar_is_fresh_in.
+      (* unfold evar_is_fresh_in.
       rewrite free_evars_nest_ex_aux.
       fold (evar_is_fresh_in (fresh_evar (s₂ ---> f)) s₂).
       eapply evar_fresh_in_subformula'. 2: apply set_evar_fresh_is_fresh.
-      simpl. rewrite is_subformula_of_refl. rewrite orb_true_r. auto.
+      simpl. rewrite is_subformula_of_refl. rewrite orb_true_r. auto. *)
       (* one subgoal remains *)
 
       apply and_iff_morphism.
-      rewrite pattern_interpretation_nest_ex_aux. reflexivity.
+      rewrite bevar_subst_not_occur; [eapply well_formed_closed_ex_aux_ind;
+                               try eassumption; lia|auto].
 
-      unfold nest_ex.
-      unfold evar_open. simpl_bevar_subst.
-      rewrite bevar_subst_nest_ex_aux;[reflexivity|]. simpl.
-      rewrite bevar_subst_nest_ex_aux;[reflexivity|]. simpl.
-      fold (nest_ex f). fold (nest_ex (nest_ex f)).
-      
-      
-      remember (fresh_evar (patt_equal (nest_ex (nest_ex f) $ patt_free_evar x') b0)) as x''.
+      unfold evar_open. simpl.
+
+      remember (fresh_evar (patt_equal (f $ patt_free_evar x') b0)) as x''.
 
       rewrite equal_iff_interpr_same. 2: apply M_satisfies_theory.
       simpl. rewrite pattern_interpretation_free_evar_simpl.
@@ -493,7 +502,7 @@ Section sorts.
       (*  Hx''neqx' : x'' ≠ x'
           Hx''freeinf : x'' ∉ free_evars f
        *)
-      pose proof (HB := @set_evar_fresh_is_fresh' _ (free_evars(patt_equal (nest_ex (nest_ex f) $ patt_free_evar x') b0))).
+      pose proof (HB := @set_evar_fresh_is_fresh' _ (free_evars(patt_equal (f $ patt_free_evar x') b0))).
       pose proof (Heqx''2 := Heqx'').
       unfold fresh_evar in Heqx''2.
       rewrite -Heqx''2 in HB.
@@ -503,47 +512,49 @@ Section sorts.
       apply sets.not_elem_of_union in HB. destruct HB as [HB _].
       apply sets.not_elem_of_union in HB. destruct HB as [Hx''freeinf Hx''neqx'].
       apply not_elem_of_singleton_1 in Hx''neqx'.
-      unfold nest_ex in Hx''freeinf.
-      rewrite 2!free_evars_nest_ex_aux in Hx''freeinf.
 
       (* Hx'fr : x' ∉ free_evars f *)
-      pose proof (Hx'fr := @set_evar_fresh_is_fresh _ (patt_exists_of_sort (nest_ex s₂) (patt_equal (nest_ex (nest_ex f) $ b1) b0))).
+      pose proof (Hx'fr := @set_evar_fresh_is_fresh _ (patt_exists_of_sort s₂ (patt_equal (f $ b1) b0))).
       rewrite -Heqx' in Hx'fr.
       unfold evar_is_fresh_in in Hx'fr. simpl in Hx'fr.
       rewrite !(left_id_L ∅ union) in Hx'fr.
       rewrite !(right_id_L ∅ union) in Hx'fr.
       apply sets.not_elem_of_union in Hx'fr. destruct Hx'fr as [_ Hx'fr].
       apply sets.not_elem_of_union in Hx'fr. destruct Hx'fr as [Hx'fr _].
-      rewrite 2!free_evars_nest_ex_aux in Hx'fr.
 
       rewrite {2}update_evar_val_comm.
-      { assumption. }
+      { rewrite bevar_subst_not_occur; [eapply well_formed_closed_ex_aux_ind;
+                try eassumption; lia|auto].
+        rewrite <- Hfreq, <- Heqx''. assumption. }
       (* do 2 rewrite -> evar_open_bound_evar. *)
       (* repeat case_match; try lia. *)
       (* rewrite <- Heqx''. *)
       (*apply Hx''neqx'.*)
       rewrite update_evar_val_same.
-      unfold nest_ex.
-      rewrite bevar_subst_nest_ex_aux.
-      { reflexivity. }
       simpl.
-      fold (nest_ex f). fold (nest_ex (nest_ex f)).
-
-      unfold nest_ex.
-      rewrite 2!pattern_interpretation_nest_ex_aux.
 
       rewrite pattern_interpretation_free_evar_independent.
-      { assumption. }
+      { rewrite bevar_subst_not_occur; [eapply well_formed_closed_ex_aux_ind;
+                try eassumption; lia|auto]. 
+        rewrite bevar_subst_not_occur; [eapply well_formed_closed_ex_aux_ind;
+                try eassumption; lia|auto]. 
+        rewrite <- Hfreq, <- Heqx''. assumption. }
       (*
       do 2 rewrite evar_open_bound_evar.
       repeat case_match; try lia.
       unfold nest_ex in Heqx''.
       rewrite <- Heqx''. assumption.*)
-      rewrite pattern_interpretation_free_evar_independent. assumption.
-      auto.
+      rewrite pattern_interpretation_free_evar_independent.
+      all: rewrite bevar_subst_not_occur; auto. 
+      all: rewrite bevar_subst_not_occur; [eapply well_formed_closed_ex_aux_ind;
+              try eassumption; lia|auto].
+      eapply evar_is_fresh_in_richer. 2: apply set_evar_fresh_is_fresh.
+      cbn. apply union_subseteq_r.
     Qed.
 
     Lemma interp_partial_function f s₁ s₂ ρₑ ρₛ :
+      well_formed_closed_ex_aux s₁ 0 -> well_formed_closed_ex_aux s₂ 0 ->
+      well_formed_closed_ex_aux f 0 ->
       @pattern_interpretation Σ M ρₑ ρₛ (patt_partial_function f s₁ s₂) = ⊤ <->
       ∀ (m₁ : Domain M),
         m₁ ∈ Minterp_inhabitant s₁ ρₑ ρₛ ->
@@ -552,27 +563,26 @@ Section sorts.
           (app_ext (@pattern_interpretation Σ M ρₑ ρₛ f) {[m₁]})
             ⊆ {[m₂]}.
     Proof.
-      rewrite pattern_interpretation_forall_of_sort_predicate.
+      intros WF1 WF2 WFF.
+      rewrite pattern_interpretation_forall_of_sort_predicate; auto.
       2: { eauto. }
 
       unfold evar_open. simpl_bevar_subst.                                                       
-      remember (fresh_evar (patt_exists_of_sort (nest_ex s₂) (patt_subseteq ((nest_ex (nest_ex f)) $ b1) b0))) as x'.
-      rewrite [nest_ex s₂]/nest_ex.
-      rewrite bevar_subst_nest_ex_aux.
-      { reflexivity. }
-      simpl.
-      rewrite -/(nest_ex s₂).
+      remember (fresh_evar (patt_exists_of_sort s₂ (patt_subseteq ( f $ b1) b0))) as x'.
 
       apply all_iff_morphism.
       unfold pointwise_relation. intros m₁.
       apply all_iff_morphism. unfold pointwise_relation. intros Hinh1.
       
-      rewrite pattern_interpretation_exists_of_sort_predicate.
+      rewrite pattern_interpretation_exists_of_sort_predicate; auto.
       2: {
         unfold evar_open. simpl_bevar_subst.
         apply T_predicate_subseteq; apply M_satisfies_theory.
       }
-      
+      2: {
+        rewrite bevar_subst_not_occur; [eapply well_formed_closed_ex_aux_ind;
+                [ | exact WF2 ] |auto]; lia. 
+      }
       apply ex_iff_morphism. unfold pointwise_relation. intros m₂.
 
       unfold Minterp_inhabitant.
@@ -580,41 +590,19 @@ Section sorts.
       rewrite 2!pattern_interpretation_sym_simpl.
       rewrite pattern_interpretation_free_evar_independent.
       {
-        fold (evar_is_fresh_in x' (nest_ex s₂)).
-
-        assert (Hfreq: x' = fresh_evar (patt_imp s₂ (nest_ex (nest_ex f)))).
-        { rewrite Heqx'. unfold fresh_evar. apply f_equal. simpl.
-          rewrite 2!free_evars_nest_ex_aux.
-          rewrite !(left_id_L ∅ union). rewrite !(right_id_L ∅ union).
-          reflexivity.
-        }
-
-        rewrite Hfreq.
-        unfold nest_ex.
-        unfold evar_is_fresh_in.
-        rewrite free_evars_nest_ex_aux.
-        fold (evar_is_fresh_in (fresh_evar (s₂ ---> f)) s₂).
-        eapply evar_fresh_in_subformula'. 2: apply set_evar_fresh_is_fresh.
-        simpl. rewrite is_subformula_of_refl. rewrite orb_true_r. auto.
+         rewrite bevar_subst_not_occur; [eapply well_formed_closed_ex_aux_ind;
+                try eassumption; lia|auto].
+         rewrite Heqx'. eapply evar_is_fresh_in_richer. 2: apply set_evar_fresh_is_fresh.
+         cbn. rewrite !(left_id_L ∅ union). rewrite !(right_id_L ∅ union). apply union_subseteq_l.
       }
-
       apply and_iff_morphism.
-      rewrite pattern_interpretation_nest_ex_aux. reflexivity.
-
-      unfold nest_ex.
-      unfold evar_open. simpl_bevar_subst.
-      rewrite bevar_subst_nest_ex_aux.
-      { reflexivity. }
-      simpl.
-      rewrite bevar_subst_nest_ex_aux.
-      { reflexivity. }
-      simpl.
-      fold (nest_ex f). fold (nest_ex (nest_ex f)).
+      rewrite bevar_subst_not_occur; [eapply well_formed_closed_ex_aux_ind;
+                [ | exact WF2 ] |auto]; lia.
       
       
-      remember (fresh_evar (patt_subseteq (nest_ex (nest_ex f) $ patt_free_evar x') b0)) as x''.
+      remember (fresh_evar (patt_subseteq (f $ patt_free_evar x') b0)) as x''.
 
-      rewrite subseteq_iff_interpr_subseteq. 2: apply M_satisfies_theory.
+      rewrite subseteq_iff_interpr_subseteq. fold bevar_subst. 2: apply M_satisfies_theory.
       simpl. rewrite pattern_interpretation_free_evar_simpl.
       rewrite update_evar_val_same.
       rewrite pattern_interpretation_app_simpl.
@@ -623,7 +611,7 @@ Section sorts.
       (*  Hx''neqx' : x'' ≠ x'
           Hx''freeinf : x'' ∉ free_evars f
        *)
-      pose proof (HB := @set_evar_fresh_is_fresh' _ (free_evars(patt_subseteq (nest_ex (nest_ex f) $ patt_free_evar x') b0))).
+      pose proof (HB := @set_evar_fresh_is_fresh' _ (free_evars(patt_subseteq (f $ patt_free_evar x') b0))).
       pose proof (Heqx''2 := Heqx'').
       unfold fresh_evar in Heqx''2.
       rewrite -Heqx''2 in HB.
@@ -632,55 +620,59 @@ Section sorts.
       rewrite !(right_id_L ∅ union) in HB.
       apply sets.not_elem_of_union in HB. destruct HB as [Hx''freeinf Hx''neqx'].
       apply not_elem_of_singleton_1 in Hx''neqx'.
-      unfold nest_ex in Hx''freeinf.
-      rewrite 2!free_evars_nest_ex_aux in Hx''freeinf.
 
       (* Hx'fr : x' ∉ free_evars f *)
-      pose proof (Hx'fr := @set_evar_fresh_is_fresh _ (patt_exists_of_sort (nest_ex s₂) (patt_subseteq (nest_ex (nest_ex f) $ b1) b0))).
+      pose proof (Hx'fr := @set_evar_fresh_is_fresh _ (patt_exists_of_sort s₂ (patt_subseteq (f $ b1) b0))).
       rewrite -Heqx' in Hx'fr.
       unfold evar_is_fresh_in in Hx'fr. simpl in Hx'fr.
       rewrite !(left_id_L ∅ union) in Hx'fr.
       rewrite !(right_id_L ∅ union) in Hx'fr.
       apply sets.not_elem_of_union in Hx'fr. destruct Hx'fr as [_ Hx'fr].
-      rewrite 2!free_evars_nest_ex_aux in Hx'fr.
       
       rewrite {2}update_evar_val_comm.
-      { assumption. }
+      { rewrite bevar_subst_not_occur; [eapply well_formed_closed_ex_aux_ind;
+                [ | exact WFF ] |auto]. lia. rewrite <- Heqx''. assumption. }
       (*do 2 rewrite evar_open_bound_evar. cbn.
       repeat case_match; try lia.
       rewrite <- Heqx''. apply Hx''neqx'. *)
       rewrite update_evar_val_same.
-      unfold nest_ex.
-      rewrite bevar_subst_nest_ex_aux;[reflexivity|]. simpl.
-      fold (nest_ex f). fold (nest_ex (nest_ex f)).
-
-      unfold nest_ex.
-      rewrite 2!pattern_interpretation_nest_ex_aux.
 
       rewrite pattern_interpretation_free_evar_independent.
-      { assumption. }
+      { rewrite bevar_subst_not_occur; [eapply well_formed_closed_ex_aux_ind;
+                [ | exact WFF ] |auto]. lia.
+        rewrite bevar_subst_not_occur; [eapply well_formed_closed_ex_aux_ind;
+                [ | exact WFF ] |auto]. lia.
+        eapply evar_is_fresh_in_richer. 2: apply set_evar_fresh_is_fresh.
+         cbn. rewrite !(left_id_L ∅ union). rewrite !(right_id_L ∅ union). apply union_subseteq_l.
+      }
       (*do 2 rewrite evar_open_bound_evar. cbn. unfold nest_ex in Heqx''.
       repeat case_match; try lia.
       rewrite <- Heqx''. assumption.*)
-      rewrite pattern_interpretation_free_evar_independent. assumption.
-      auto.
+      rewrite pattern_interpretation_free_evar_independent.
+      all: rewrite bevar_subst_not_occur; [eapply well_formed_closed_ex_aux_ind;
+               try eassumption |auto].
+      2,5: rewrite bevar_subst_not_occur; [eapply well_formed_closed_ex_aux_ind;
+               try eassumption |auto].
+      3, 5: exact WFF. all: try lia.
+      all: rewrite bevar_subst_not_occur; [eapply well_formed_closed_ex_aux_ind;
+               try eassumption |auto]; lia.
     Qed.
 
-    Lemma Minterp_inhabitant_evar_open_update_evar_val ρₑ ρₛ x e s m:
-      evar_is_fresh_in x s ->
-      m ∈ Minterp_inhabitant (evar_open 0 x (nest_ex s)) (update_evar_val x e ρₑ) ρₛ
+    Lemma Minterp_inhabitant_evar_open_update_evar_val ρₑ ρₛ x e s m n:
+      evar_is_fresh_in x s -> well_formed_closed_ex_aux s n ->
+      m ∈ Minterp_inhabitant (evar_open n x s) (update_evar_val x e ρₑ) ρₛ
       <-> m ∈ Minterp_inhabitant s ρₑ ρₛ.
     Proof.
-      intros Hfr.
+      intros Hfr Hwf.
       unfold Minterp_inhabitant.
       rewrite 2!pattern_interpretation_app_simpl.
       rewrite 2!pattern_interpretation_sym_simpl.
-      rewrite pattern_interpretation_evar_open_nest_ex.
-      { exact Hfr. }
-      auto.
+      unfold evar_open. rewrite bevar_subst_not_occur; [ auto | ].
+      rewrite pattern_interpretation_free_evar_independent; [solve_free_evars_inclusion 5 | ]; auto.
    Qed.
-    
+
     Lemma interp_partial_function_injective f s ρₑ ρₛ :
+      well_formed_closed_ex_aux s 0 -> well_formed_closed_ex_aux f 0 ->
       @pattern_interpretation Σ M ρₑ ρₛ (patt_partial_function_injective f s) = ⊤ <->
       ∀ (m₁ : Domain M),
         m₁ ∈ Minterp_inhabitant s ρₑ ρₛ ->
@@ -690,8 +682,9 @@ Section sorts.
           (rel_of ρₑ ρₛ f) m₁ = (rel_of ρₑ ρₛ f) m₂ ->
           m₁ = m₂.
     Proof.
+      intros WfS WfF.
       unfold patt_partial_function_injective.
-      rewrite pattern_interpretation_forall_of_sort_predicate.
+      rewrite pattern_interpretation_forall_of_sort_predicate; auto.
       2: {
         match goal with
         | [ |- M_predicate _ (evar_open _ ?x _) ] => remember x
@@ -706,91 +699,53 @@ Section sorts.
       }
       remember
       (fresh_evar
-               (patt_forall_of_sort (nest_ex s)
-                  (! patt_equal (nest_ex (nest_ex f) $ b1) Bot --->
-                     patt_equal (nest_ex (nest_ex f) $ b1) (nest_ex (nest_ex f) $ b0) ---> patt_equal b1 b0)))
+               (patt_forall_of_sort  s
+                  (! patt_equal ( f $ b1) Bot --->
+                     patt_equal ( f $ b1) ( f $ b0) ---> patt_equal b1 b0)))
       as x₁.
       apply all_iff_morphism. intros m₁.
       apply all_iff_morphism. intros Hm₁s.
 
       unfold evar_open. simpl_bevar_subst.
       rewrite pattern_interpretation_forall_of_sort_predicate. 2: { eauto 8. }
-      rewrite [0+1]/=.
+      2: { rewrite bevar_subst_not_occur; auto.
+           eapply well_formed_closed_ex_aux_ind. 2: exact WfS. lia.
+      }
       remember
       (fresh_evar
                (evar_open 1 x₁
-                  (! patt_equal (nest_ex (nest_ex f) $ b1) Bot --->
-                     patt_equal (nest_ex (nest_ex f) $ b1) (nest_ex (nest_ex f) $ b0) ---> patt_equal b1 b0)))
+                  (! patt_equal (f $ b1) Bot --->
+                     patt_equal (f $ b1) (f $ b0) ---> patt_equal b1 b0)))
       as x₂.
         
-      apply all_iff_morphism. intros m₂.
+      apply all_iff_morphism. intros m₂. simpl.
       rewrite Minterp_inhabitant_evar_open_update_evar_val.
-      2: {
-        eapply evar_is_fresh_in_richer.
-        2: { subst x₁.
-             apply set_evar_fresh_is_fresh.
-        }
-        solve_free_evars_inclusion 5.
-      }
+      repeat rewrite bevar_subst_not_occur; auto.
+      1,4: eapply well_formed_closed_ex_aux_ind; try eassumption; lia.
+      2: { rewrite Heqx₁. eapply evar_is_fresh_in_richer. 2: apply set_evar_fresh_is_fresh.
+           cbn. rewrite !(left_id_L ∅ union). rewrite !(right_id_L ∅ union). apply union_subseteq_l. }
       apply all_iff_morphism. intros Hm₂s.
       unfold evar_open. simpl_bevar_subst.
 
       rewrite pattern_interpretation_predicate_impl. 2: { eauto. }
       simpl.
-      rewrite pattern_interpretation_predicate_not. 2: { eauto. }
+      rewrite pattern_interpretation_predicate_not. 2: { rewrite bevar_subst_not_occur; auto. eauto. }
       rewrite equal_iff_interpr_same.
       rewrite pattern_interpretation_bott_simpl. 2: apply M_satisfies_theory.
-      rewrite bevar_subst_nest_ex_aux;[reflexivity|]. simpl.
+
+      repeat rewrite bevar_subst_not_occur; auto. simpl.
       rewrite pattern_interpretation_app_simpl.
-      fold (nest_ex (evar_open 0 x₁ (nest_ex f))).
-      rewrite pattern_interpretation_evar_open_nest_ex.
-      {
-        eapply evar_is_fresh_in_richer. 2: { subst. apply set_evar_fresh_is_fresh. }
-        unfold evar_open. simpl.
-        fold (evar_open 1 
-             (fresh_evar
-                (patt_forall_of_sort (nest_ex s)
-                   (! patt_equal (nest_ex (nest_ex f) $ b1) ⊥ --->
-                    patt_equal (nest_ex (nest_ex f) $ b1)
-                      (nest_ex (nest_ex f) $ b0) ---> 
-                    patt_equal b1 b0))) (nest_ex (nest_ex f))).
-        fold (evar_open 0 x₁ (nest_ex f)).
-        solve_free_evars_inclusion 5.
-      }
-      rewrite pattern_interpretation_evar_open_nest_ex.
-      {
-        eapply evar_is_fresh_in_richer. 2: { subst. apply set_evar_fresh_is_fresh. }
-        solve_free_evars_inclusion 4.
-      }
       rewrite pattern_interpretation_free_evar_simpl.
       rewrite update_evar_val_neq.
       { solve_fresh_neq. }
       rewrite update_evar_val_same.
       fold (rel_of ρₑ ρₛ f m₁).
-      apply all_iff_morphism. unfold pointwise_relation. intros Hnonempty.
+      (* apply all_iff_morphism. unfold pointwise_relation. intros Hnonempty. *)
 
       rewrite pattern_interpretation_predicate_impl. 2: { eauto. }
       (*rewrite simpl_evar_open.*)
       rewrite equal_iff_interpr_same. 2: apply M_satisfies_theory.
       rewrite 2!pattern_interpretation_app_simpl.
-      rewrite !pattern_interpretation_evar_open_nest_ex.
-      {
-        eapply evar_is_fresh_in_richer. 2: { subst. apply set_evar_fresh_is_fresh. }
-        unfold evar_open. simpl.
-        fold (evar_open 1 
-             (fresh_evar
-                (patt_forall_of_sort (nest_ex s)
-                   (! patt_equal (nest_ex (nest_ex f) $ b1) ⊥ --->
-                    patt_equal (nest_ex (nest_ex f) $ b1)
-                      (nest_ex (nest_ex f) $ b0) ---> 
-                    patt_equal b1 b0))) (nest_ex (nest_ex f))).
-        fold (evar_open 0 x₁ (nest_ex f)).
-        solve_free_evars_inclusion 4.
-      }
-      {
-        eapply evar_is_fresh_in_richer. 2: { subst. apply set_evar_fresh_is_fresh. }
-        solve_free_evars_inclusion 4.
-      }
       rewrite equal_iff_interpr_same. 2: { apply M_satisfies_theory. }
       rewrite !pattern_interpretation_free_evar_simpl.
       rewrite update_evar_val_same.
@@ -798,15 +753,21 @@ Section sorts.
       { solve_fresh_neq. }
       rewrite update_evar_val_same.
       unfold rel_of.
-      apply all_iff_morphism. intros Hfm1eqfm2.
-      clear.
-      set_solver.
+      repeat rewrite pattern_interpretation_free_evar_independent.
+      3: apply all_iff_morphism; intros Hfm1eqfm2; clear; set_solver.
+      { eapply evar_is_fresh_in_richer. 2: apply set_evar_fresh_is_fresh.
+        cbn. rewrite !(left_id_L ∅ union). rewrite !(right_id_L ∅ union).
+        clear. set_solver.
+      }
+      { rewrite Heqx₁. clear. eapply evar_is_fresh_in_richer. 2: apply set_evar_fresh_is_fresh. set_solver. }
     Qed.
 
     Lemma interp_total_function_injective f s ρₑ ρₛ :
+      well_formed_closed_ex_aux s 0 -> well_formed_closed_ex_aux f 0 ->
       @pattern_interpretation Σ M ρₑ ρₛ (patt_total_function_injective f s) = ⊤ <->
       total_function_is_injective f (Minterp_inhabitant s ρₑ ρₛ) ρₑ ρₛ.
     Proof.
+      intros WfS WfF.
       unfold total_function_is_injective.
       unfold patt_partial_function_injective.
       rewrite pattern_interpretation_forall_of_sort_predicate.
@@ -824,8 +785,8 @@ Section sorts.
       }
       remember
       (fresh_evar
-               (patt_forall_of_sort (nest_ex s)
-                  (patt_equal (nest_ex (nest_ex f) $ b1) (nest_ex (nest_ex f) $ b0) ---> patt_equal b1 b0)))
+               (patt_forall_of_sort s
+                  (patt_equal (f $ b1) (f $ b0) ---> patt_equal b1 b0)))
       as x₁.
       apply all_iff_morphism. intros m₁.
       apply all_iff_morphism. intros Hm₁s.
@@ -839,13 +800,12 @@ Section sorts.
         unfold evar_open. simpl_bevar_subst. simpl.
         eauto.
       }
-      rewrite [0+1]/=.
       remember
       (fresh_evar
                (evar_open 1 x₁
-                  (patt_equal (nest_ex (nest_ex f) $ b1) (nest_ex (nest_ex f) $ b0) ---> patt_equal b1 b0)))
+                  (patt_equal (f $ b1) (f $ b0) ---> patt_equal b1 b0)))
       as x₂.
-        
+
       apply all_iff_morphism. intros m₂.
       rewrite Minterp_inhabitant_evar_open_update_evar_val.
       2: {        
@@ -861,26 +821,7 @@ Section sorts.
       
       rewrite equal_iff_interpr_same.
       2: { apply M_satisfies_theory. }
-      rewrite bevar_subst_nest_ex_aux;[reflexivity|]. simpl.
-      fold (nest_ex (evar_open 0 x₁ (nest_ex f))).
       rewrite 2!pattern_interpretation_app_simpl.
-      rewrite pattern_interpretation_evar_open_nest_ex.
-      {
-        eapply evar_is_fresh_in_richer. 2: { subst. apply set_evar_fresh_is_fresh. }
-        unfold evar_open. simpl.
-        fold (evar_open 1 
-             (fresh_evar
-             (patt_forall_of_sort (nest_ex s)
-                (patt_equal (nest_ex (nest_ex f) $ b1) (nest_ex (nest_ex f) $ b0) --->
-                 patt_equal b1 b0))) (nest_ex (nest_ex f))).
-        fold (evar_open 0 x₁ (nest_ex f)).
-        solve_free_evars_inclusion 5.
-      }
-      rewrite pattern_interpretation_evar_open_nest_ex.
-      {
-        eapply evar_is_fresh_in_richer. 2: { subst. apply set_evar_fresh_is_fresh. }
-        solve_free_evars_inclusion 4.
-      }
       rewrite pattern_interpretation_free_evar_simpl.
       rewrite update_evar_val_neq.
       { solve_fresh_neq. }
@@ -889,7 +830,10 @@ Section sorts.
       rewrite pattern_interpretation_free_evar_simpl.
       rewrite update_evar_val_same.
       fold (rel_of ρₑ ρₛ f m₁). fold (rel_of ρₑ ρₛ f m₂).
-      apply all_iff_morphism. intros Hfm1eqfm2.
+
+      repeat rewrite bevar_subst_not_occur; auto; simpl.
+      { eapply well_formed_closed_ex_aux_ind. 2: eassumption. lia. }
+      
 
 
       rewrite equal_iff_interpr_same. 2: apply M_satisfies_theory.
@@ -898,7 +842,13 @@ Section sorts.
       rewrite update_evar_val_neq.
       { solve_fresh_neq. }
       rewrite update_evar_val_same.
+      repeat rewrite pattern_interpretation_free_evar_independent.
+      1-2: rewrite Heqx₁; clear; eapply evar_is_fresh_in_richer; [|apply set_evar_fresh_is_fresh]; set_solver.
+      apply all_iff_morphism. intros Hfm1eqfm2.
       clear. set_solver.
+      { eapply well_formed_closed_ex_aux_ind. 2: eassumption. lia. }
+      { rewrite bevar_subst_not_occur; auto; simpl. eapply well_formed_closed_ex_aux_ind. 2: eassumption. lia. }
+      { auto. }
     Qed.
 
 
